CCsub_Lemmas.v
@@ -44,30 +44,19 @@ Qed.
 
 Lemma notin_fv_tt_open_tt_rec : forall k (X : atom) U T,
   X `notin` fv_tt (open_tt_rec k U T) ->
-  X `notin` fv_tt T
-with notin_fv_tpt_open_tpt_rec : forall k (X : atom) U T,
-  X `notin` fv_tpt (open_tpt_rec k U T) ->
-  X `notin` fv_tpt T.
+  X `notin` fv_tt T.
 Proof.
-------
   intros k X U T. unfold open_tt.
   generalize k.
   induction T; simpl; intros k0 Fr; notin_simpl; try apply notin_union; eauto.
-------
-  intros k X U T. unfold open_tt.
-  generalize k.
-  induction T; simpl; intros k0 Fr; notin_simpl; try apply notin_union; eauto.
+  unfold open_vt in Fr; destruct v; simpl in Fr; fsetdec.
 Qed.
 
 Lemma notin_fv_tt_open_tt : forall (X : atom) U T,
   X `notin` fv_tt (open_tt T U) ->
-  X `notin` fv_tt T
-with notin_fv_tpt_open_tpt : forall (X : atom) U T,
-  X `notin` fv_tpt (open_tpt T U) ->
-  X `notin` fv_tpt T.
+  X `notin` fv_tt T.
 Proof with eauto.
   intros. apply notin_fv_tt_open_tt_rec with (k := 0) (U := U)...
-  intros. apply notin_fv_tpt_open_tpt_rec with (k := 0) (U := U)...
 Qed.
 
 Lemma notin_cset_fvars_open_cset : forall X k C c,
@@ -83,58 +72,34 @@ Qed.
 
 Lemma notin_fv_tt_open_ct_rec : forall k (X : atom) C T,
   X `notin` fv_tt (open_ct_rec k C T) ->
-  X `notin` fv_tt T
-with notin_fv_tt_open_cpt_rec : forall k (X : atom) C P,
-  X `notin` fv_tpt (open_cpt_rec k C P) ->
-  X `notin` fv_tpt P.
+  X `notin` fv_tt T.
 Proof with eauto using notin_cset_fvars_open_cset.
-------
   intros k Y C T. unfold open_tt.
   generalize k.
   induction T; simpl; intros k0 Fr; notin_simpl; try apply notin_union; eauto.
-------
-  intros k Y C P. unfold open_tt.
-  generalize k.
-  induction P; simpl; intros k0 Fr; notin_simpl; try apply notin_union; eauto.
 Qed.
 
 Lemma notin_fv_tt_open_ct : forall (X : atom) C T,
   X `notin` fv_tt (open_ct T C) ->
-  X `notin` fv_tt T
-with notin_fv_tpt_open_cpt : forall (X : atom) C T,
-  X `notin` fv_tpt (open_cpt T C) ->
-  X `notin` fv_tpt T.
+  X `notin` fv_tt T.
 Proof with eauto.
   intros. apply notin_fv_tt_open_ct_rec with (k := 0) (C := C)...
-  intros. apply notin_fv_tt_open_cpt_rec with (k := 0) (C := C)...
 Qed.
 
 Lemma notin_fv_ct_open_tt_rec : forall k (X : atom) U T,
   X `notin` fv_ct (open_tt_rec k U T) ->
-  X `notin` fv_ct T
-with notin_fv_cpt_open_tpt_rec : forall k (X : atom) U P,
-  X `notin` fv_cpt (open_tpt_rec k U P) ->
-  X `notin` fv_cpt P.
+  X `notin` fv_ct T.
 Proof with eauto using notin_cset_fvars_open_cset.
-------
   intros k X U T. unfold open_tt.
   generalize k.
   induction T; simpl; intros k0 Fr; notin_simpl; try apply notin_union...
-------
-  intros k X U P. unfold open_tt.
-  generalize k.
-  induction P; simpl; intros k0 Fr; notin_simpl; try apply notin_union; eauto.
 Qed.
 
 Lemma notin_fv_ct_open_tt : forall (X : atom) U T,
   X `notin` fv_ct (open_tt T U) ->
-  X `notin` fv_ct T
-with notin_fv_cpt_open_tpt : forall (X : atom) U P,
-  X `notin` fv_cpt (open_tpt P U) ->
-  X `notin` fv_cpt P.
+  X `notin` fv_ct T.
 Proof with eauto*.
   intros. apply notin_fv_ct_open_tt_rec with (k := 0) (U := U)...
-  intros. apply notin_fv_cpt_open_tpt_rec with (k := 0) (U := U)...
 Qed.
 
 Lemma notin_fv_tt_open : forall (X : atom) U T,
@@ -149,34 +114,23 @@ Qed.
 
 Lemma notin_fv_ct_open_ct_rec : forall (X : atom) T C k,
   X `notin` fv_ct (open_ct_rec k C T) ->
-  X `notin` fv_ct T
-with notin_fv_ct_open_cpt_rec : forall (X : atom) T C k,
-  X `notin` fv_cpt (open_cpt_rec k C T) ->
-  X `notin` fv_cpt T.
+  X `notin` fv_ct T.
 Proof with auto.
-------
   intros X T C.
   induction T ; simpl ; intros k Fr ; try apply notin_union; eauto.
+  - apply IHT1 with (k := k)...
+  - apply IHT2 with (k := S k)...
+  - apply IHT1 with (k := k)...
+  - apply IHT2 with (k := S k)... 
   - apply notin_cset_fvars_open_cset with (k := k) (C := C)...
-  - apply notin_fv_ct_open_cpt_rec with (C := C) (k := k)...
-------
-    intros X T C.
-    induction T ; simpl ; intros k Fr ; try apply notin_union; eauto.
-    - apply notin_fv_ct_open_ct_rec with (C := C) (k := k)...
-    - apply notin_fv_ct_open_ct_rec with (C := C) (k := S k)...
-    - apply notin_fv_ct_open_ct_rec with (C := C) (k := k)...
-    - apply notin_fv_ct_open_ct_rec with (C := C) (k := S k)...
+  - apply IHT with (k := k)...
 Qed.
 
 Lemma notin_fv_ct_open_ct : forall (X : atom) T C,
   X `notin` fv_ct (open_ct T C) ->
-  X `notin` fv_ct T
-with notin_fv_ct_open_cpt : forall (X : atom) T C,
-  X `notin` fv_cpt (open_cpt T C) ->
-  X `notin` fv_cpt T.
+  X `notin` fv_ct T.
 Proof with auto.
   intros. apply notin_fv_ct_open_ct_rec with (k := 0) (C := C)...
-  intros. apply notin_fv_ct_open_cpt_rec with (k := 0) (C := C)...
 Qed.
 
 (* Lemma notin_fv_ct_open_ct_rec : forall (Y X : atom) T k, *)
@@ -227,64 +181,48 @@ Proof with auto.
   - apply notin_fv_ct_open_ct with (C := C)...
 Qed.
 
-Lemma notin_fv_wf_typ : forall E Ap Am (X : atom) T,
-  wf_typ E Ap Am T ->
-  X `notin` dom E ->
-  X `notin` (fv_tt T `union` fv_ct T)
-with notin_fv_wf_pretyp : forall E Ap Am (X : atom) T,
-  wf_pretyp E Ap Am T ->
-  X `notin` dom E ->
-  X `notin` (fv_tpt T `union` fv_cpt T).
+Lemma notin_fv_wf_typ : forall Γ (X : atom) T,
+  Γ ⊢ T wf ->
+  X `notin` dom Γ ->
+  X `notin` (fv_tt T `union` fv_ct T).
 Proof with eauto.
--------
-  intros * Wf_typ.
-  induction Wf_typ; intros FrE; simpl.
-  - assert (X0 `in` dom E) by (eapply binds_In; eauto)...
-  - specialize (notin_fv_wf_pretyp _ _ _ _ _ H0 FrE) as Wf.
-    inversion H; destruct C; subst; simpl in *; try notin_solve.
-    assert (X `notin` fvars)... {
-      unfold allbound in *.
-      intro Hin; specialize (H1 X Hin) as [T B].
-      destruct_bound B; apply binds_In in B...
-    }
--------
-  intros * Wf_pretyp.
-  induction Wf_pretyp; intros FrE; simpl. (* do not add automation, takes excessive time *)
-  - fsetdec.
-  - pick fresh Y.
-    specialize (notin_fv_wf_typ _ _ _ X _ H ltac:(assumption)) as HT1.
-    specialize (H0 Y ltac:(notin_solve)) as WfT2.
-    specialize (notin_fv_wf_typ _ _ _ X _ WfT2) as HT2.
-    simpl in *.
-    specialize (HT2 ltac:(notin_solve)).
-    assert (X `notin` fv_tt T2). {
-      apply notin_fv_tt_open_ct with (C := (`cset_fvar` Y))...
-    }
-    assert (X `notin` fv_ct T2);
-      [ apply notin_fv_ct_open_ct with (C := (`cset_fvar` Y)); try discriminate | .. ]...
-  - pick fresh Y.
-    specialize (notin_fv_wf_typ _ _ _ X _ H ltac:(assumption)) as HT1.
-    specialize (H0 Y ltac:(notin_solve)) as WfT2.
-    specialize (notin_fv_wf_typ _ _ _ X _ WfT2) as HT2.
-    simpl in *.
-    specialize (HT2 ltac:(notin_solve)).
-    assert (X `notin` fv_tt T2). {
-      apply notin_fv_tt_open_tt with (U := Y)...
-    }
-    assert (X `notin` fv_ct T2);
-      [ apply notin_fv_ct_open_tt with (U := Y); try discriminate | .. ]...
-Qed.
-
-Lemma notin_fv_wf : forall E (X : atom) T,
-  wf_typ_in E T ->
-  X `notin` dom E ->
-  X `notin` fv_tt T.
-Proof with eauto.
-  intros E X T Wf_typ F.
-  assert (X `notin` (fv_tt T `union` fv_ct T)). {
-    eapply notin_fv_wf_typ...
-  }
-  fsetdec.
+  intros * WfT.
+  induction WfT; intros FrE; simpl.
+  - Case "X0".
+    enough (X <> X0) by fsetdec.
+    enough (X0 ∈ dom Γ) by fsetdec.
+    applys binds_In H.
+  - Case "⊤".
+    fsetdec.
+  - Case "∀ (S) T".
+    pick fresh y.
+    specialize (H0 y ltac:(fsetdec)).
+    rewrite dom_concat in H0; simpl in H0.
+    specialize (H0 ltac:(notin_solve)).
+    destruct (AtomSetNotin.elim_notin_union H0) as [H1 H2].
+    apply notin_fv_tt_open_ct in H1.
+    apply notin_fv_ct_open_ct in H2.
+    specialize (IHWfT ltac:(notin_solve)).
+    clear - H1 H2 IHWfT.
+    fsetdec.
+  - Case "∀ [R] T".
+    pick fresh Y.
+    specialize (H1 Y ltac:(fsetdec)).
+    rewrite dom_concat in H1; simpl in H1.
+    specialize (H1 ltac:(notin_solve)).
+    destruct (AtomSetNotin.elim_notin_union H1) as [H2 H3].
+    apply notin_fv_tt_open_tt in H2.
+    apply notin_fv_ct_open_tt in H3.
+    specialize (IHWfT ltac:(notin_solve)).
+    clear - H2 H3 IHWfT.
+    fsetdec.
+  - Case "□ T".
+    auto.
+  - Case "C # R".
+    specialize (IHWfT FrE).
+    destruct H.
+    enough (X `notin` fvars) by fsetdec.
+    fsetdec.
 Qed.
 
 Local Lemma notin_fv_vv_open_vv : forall k u x v,
@@ -304,6 +242,7 @@ Proof with eauto using notin_fv_vv_open_vv.
   intros. generalize dependent k.
   induction t; simpl in *; intros k H; try (trivial || notin_solve)...
   all: destruct (AtomSetNotin.elim_notin_union H)...
+  destruct v; simpl in *; enough (x ∉ `cset_fvars` c) by fsetdec; eapply notin_cset_fvars_open_cset...
 Qed.
 
 Lemma notin_fv_ve_open_ve : forall u (y x : atom) t,
@@ -339,7 +278,9 @@ Local Lemma notin_fv_ve_open_te_rec : forall k (y x : atom) t,
 Proof with eauto.
   intros. generalize dependent k.
   induction t; simpl in *; intros k H; try (trivial || notin_solve)...
-  destruct (AtomSetNotin.elim_notin_union H)...
+  all: destruct (AtomSetNotin.elim_notin_union H)...
+  enough (x ∉ `cset_fvars` c) by fsetdec.
+  eapply notin_cset_fvars_open_cset...
 Qed.
 
 Lemma notin_fv_ve_open_te : forall (y x : atom) t,
@@ -368,14 +309,137 @@ Qed.
 (** * #<a name="cvfree"></a># Lemmas about free variables -- in particular properties of [free_for_cv] *)
 (** TODO Maybe have a separate file for free_for_cv lemmas **)
 
-Lemma cv_free_never_universal : forall e,
-  ~ `* in` (free_for_cv e).
+(* REVIEW: none of these are true anymore, since exp_cv could be universal.
+
+Lemma exp_cv_open_ve_rec_same_uvar : forall k x C e,
+  `cset_uvar` (exp_cv (open_ve_rec k x C e)) = `cset_uvar` (exp_cv e).
 Proof with eauto*.
-  intros. induction e; repeat match goal with [v : var |- _] => destruct v; simpl; eauto* end; try discriminate...
+  intros.
+  revert k.
+  induction e; intros k; simpl.
+  - destruct v; simpl in *...
+    destruct (k === n)...
+  - apply IHe.
+  - destruct v; simpl.
+    + destruct v0; simpl.
+      * reflexivity.
+      * destruct (k === n); simpl...
+    + destruct v0; simpl.
+      * destruct (k === n); simpl...
+      * destruct (k === n); destruct (k === n0); simpl...
+  - f_equal.
+    + apply IHe1.
+    + apply IHe2.
+  - apply IHe.
+  - destruct v; simpl.
+    + reflexivity.
+    + destruct (k === n); simpl...
+  - reflexivity.
+  - f_equal.
+    + unfold open_cset.
+      destruct_set_mem k c.
+    + destruct v; simpl.
+      * reflexivity.
+      * destruct (k === n); simpl...
+Qed.
+
+Lemma typ_cv_never_universal : forall o
+
+Lemma exp_cv_open_te_rec_same_uvar : forall k T e,
+  type T ->
+  `cset_uvar` (exp_cv (open_te_rec k T e)) = `cset_uvar` (exp_cv e).
+Proof with eauto*.
+  intros.
+  revert k.
+  induction e; intros k; simpl...
+  - f_equal.
+    + apply IHe1.
+    + apply IHe2.
+  - f_equal.
+    destruct v; simpl.
+    + unfold open_cset.
+      destruct_set_mem k c.
+    destruct v; simpl;
+      repeat rewrite orb_false_r;
+      unfold open_cset;
+      destruct_set_mem k c;
+      destruct c eqn:Hc;
+      simpl...
+    + unfold typ_cv.
+      destruct T eqn:HeqT...
+      * destruct v...
+      * exfalso.
+        inversion H; inversion H0.
+        destruct c0.
+  - destruct v; simpl in *...
+    destruct (k === n)...
+  - apply IHe.
+  - destruct v; simpl.
+    + destruct v0; simpl.
+      * reflexivity.
+      * destruct (k === n); simpl...
+    + destruct v0; simpl.
+      * destruct (k === n); simpl...
+      * destruct (k === n); destruct (k === n0); simpl...
+  - f_equal.
+    + apply IHe1.
+    + apply IHe2.
+  - apply IHe.
+  - destruct v; simpl.
+    + reflexivity.
+    + destruct (k === n); simpl...
+  - reflexivity.
+  - f_equal.
+    + unfold open_cset.
+      destruct_set_mem k c.
+    + destruct v; simpl.
+      * reflexivity.
+      * destruct (k === n); simpl...
+Qed.
+
+Lemma exp_cv_never_universal : forall e,
+  expr e ->
+  ~ `* in` (exp_cv e).
+Proof with eauto*.
+  intros.
+  induction H; simpl...
+  - pick fresh x and specialize H1.
+    erewrite <- exp_cv_open_ve_rec_same_uvar.
+    apply H1.
+  - pick fresh x and specialize H1.
+    intro.
+    destruct (`cset_uvar` (exp_cv e1)) eqn:He1...
+    destruct (`cset_uvar` (exp_cv e2)) eqn:He2...
+    erewrite <- exp_cv_open_ve_rec_same_uvar with (k := 0) (x := x) (C := `cset_fvar` x) in He2.
+    apply (H1 He2).
+  - pick fresh X and specialize H1.
+    erewrite <- exp_cv_open_te_rec_same_uvar.
+    apply H1.
+    appl 
+    destruct (exp_cv (open_ve_rec 0 x (`cset_fvar` x) e2)) eqn:Hu.
+    inversion Hu; subst.
+    assert (`cset_uvar` (exp_cv (open_ve_rec 0 x (`cset_fvar` x) e2)) = `cset_uvar` (cset_set t t0 true)).
+    { Unset Printing Notations. f_equal.
+
+    }
+    replace ( * ∈ exp_cv (open_ve_rec 0 x (`cset_fvar` x) e2)) with (`cset_uvar` (exp_cv (open_ve e2 x (`cset_fvar` x)))).
+    Unset Printing Notations.
+    
+    erewrite <- exp_cv_open_ve_rec_same_uvar.
+    enough (`cset_uvar` (exp_cv e2) = false).
+  induction H;
+    repeat match goal with
+    | [v : var |- _] =>
+        destruct v;
+        simpl;
+        eauto*
+    end;
+    try discriminate...
   simpl.
-  destruct (free_for_cv e1) eqn:Hfc1;
-  destruct (free_for_cv e2) eqn:Hfc2...
-  csetdec.
+  - destruct (exp_cv e1) eqn:Hfc1;
+    destruct (exp_cv e2) eqn:Hfc2...
+    csetdec.
+  -  
 Qed.
 
 Lemma cv_free_has_universal_false : forall e,
@@ -401,16 +465,17 @@ Proof with eauto using cv_free_var_is_bvar_free.
   - intros x. apply NatSetNotin.notin_union; apply cv_free_var_is_bvar_free.
   - intros x. apply NatSetNotin.notin_union; [ apply IHe1 | apply IHe2 ].
 Qed.
+*)
 
-Lemma cv_free_atom : forall (x : atom),
-  free_for_cv x = (`cset_fvar` x).
+Lemma exp_cv_free_atom : forall (x : atom),
+  exp_cv x = (`cset_fvar` x).
 Proof with auto*.
   intros.
-  unfold free_for_cv...
+  unfold exp_cv...
 Qed.
 
-Lemma free_for_cv_var_open : forall v k (y : atom),
-  cset_subset_prop (free_for_cv_var v) (free_for_cv_var (open_vv k y v)).
+Lemma var_cv_open : forall v k (y : atom),
+  cset_subset_prop (var_cv v) (var_cv (open_vv k y v)).
 Proof with eauto*.
   intros.
   destruct v; simpl...
@@ -420,26 +485,44 @@ Proof with eauto*.
   fsetdec.
 Qed.
 
-Lemma free_for_cv_open : forall e k (y : atom) C,
-  cset_subset_prop (free_for_cv e) (free_for_cv (open_ve_rec k y C e)).
-Proof with eauto using free_for_cv_var_open, subset_union.
+Lemma exp_cv_open_ve_rec : forall e k (y : atom) C,
+  cset_subset_prop (exp_cv e) (exp_cv (open_ve_rec k y C e)).
+Proof with eauto using var_cv_open, subset_union.
   intros e.
   induction e; intros; simpl...
+  destruct v; csetsimpl; destruct c.
+  - repeat split; unfold open_cset.
+    + destruct_set_mem k t0; simpl; fsetdec.
+    + fsetdec.
+    + destruct_set_mem k t0; simpl; fsetdec.
+  - repeat split; unfold open_cset; csetsimpl.
+    + destruct_set_mem k t0; simpl; fsetdec.
+    + destruct (k === n); simpl; fsetdec.
+    + destruct_set_mem k t0; destruct (k === n); subst; unfold leb; destruct b; simpl...
 Qed.
 
-Lemma free_for_cv_open_type : forall e k (y : atom),
-  cset_subset_prop (free_for_cv e) (free_for_cv (open_te_rec k y e)).
+Lemma exp_cv_open_te_rec : forall e k (y : atom),
+  cset_subset_prop (exp_cv e) (exp_cv (open_te_rec k y e)).
 Proof with eauto*.
   induction e; intros; simpl...
   specialize (IHe1 k y).
   specialize (IHe2 (`succ` k) y).
   apply subset_union...
+  destruct c.
+  repeat split;
+    csetsimpl;
+    destruct v;
+    unfold open_cset;
+    simpl; eauto*;
+    destruct_set_mem k t0;
+    simpl; eauto*;
+    fsetdec.
 Qed.
 
-Lemma free_for_cv_var_bound : forall E v (x : atom),
-  wf_cset_in E (free_for_cv_var v) ->
-  x A`in` (free_for_cv_var v) ->
-  exists T, bound x T E.
+Lemma var_cv_bound : forall Γ v (x : atom),
+  Γ ⊢ₛ (var_cv v) wf ->
+  x A`in` (var_cv v) ->
+  exists T, bound x T Γ.
 Proof with eauto.
   intros.
   destruct v; simpl in *.
@@ -448,165 +531,231 @@ Proof with eauto.
   - fsetdec.
 Qed.
 
-Lemma free_for_cv_bound : forall E e (x : atom),
-  wf_cset_in E (free_for_cv e) ->
-  x A`in` (free_for_cv e) ->
-  exists T, bound x T E.
-Proof with eauto using wf_cset_over_union, cv_free_never_universal, free_for_cv_var_bound.
-  intros E e.
+Lemma exp_cv_bound : forall Γ e (x : atom),
+  Γ ⊢ₛ (exp_cv e) wf ->
+  x A`in` (exp_cv e) ->
+  exists T, bound x T Γ.
+Proof with eauto using var_cv_bound.
+  intros Γ e.
   induction e; intros; simpl in *; try fsetdec...
+  - apply wf_cset_over_union in H.
+    destruct H.
+    destruct (AtomSet.F.union_1 H0)...
+  - apply wf_cset_over_union in H.
+    destruct H.
+    destruct (AtomSet.F.union_1 H0)...
   - apply wf_cset_over_union in H.
     destruct H.
     apply cset_references_fvar_over_union in H0...
     destruct H0...
-  - apply wf_cset_over_union in H...
-    apply cset_references_fvar_over_union in H0...
-    inversion H0.
-    + apply IHe1... apply H.
-    + apply IHe2... apply H.
+    inversion H; subst...
 Qed.
 
-Lemma free_for_cv_var_is_free_vv : forall v,
-  cset_subset_prop (free_for_cv_var v) (cset_set (fv_vv v) {}N false).
+Lemma var_cv_subset_fv_vv : forall v,
+  `cset_fvars` (var_cv v) `c`A fv_vv v.
 Proof with eauto.
   intros v.
-  destruct v; simpl...
+  destruct v; simpl; fsetdec.
 Qed.
 
-Lemma free_for_cv_is_free_ve : forall e,
-  cset_subset_prop (free_for_cv e) (cset_set (fv_ve e) {}N false).
-Proof with eauto using cv_free_never_universal, free_for_cv_var_is_free_vv; eauto*.
-  intros e.
+Lemma var_cv_closed : forall v,
+  `cset_bvars` (var_cv v) = {}N.
+Proof with eauto*.
+  destruct v...
+Qed.
+
+Lemma exp_cv_subset_fv_ve : forall e,
+  `cset_fvars` (exp_cv e) `c`A fv_ve e.
+Proof with eauto using var_cv_subset_fv_vv, atomset_subset_union; eauto*.
   induction e; simpl...
-  - replace (cset_set (fv_vv v `u`A fv_vv v0) {}N false) with ((cset_set (fv_vv v) {}N false) `u` (cset_set (fv_vv v0) {}N false)).
-    + apply subset_union...
-    + unfold cset_union; simpl; rewrite empty_funion_idempotent; reflexivity.
-  - replace (cset_set (fv_ve e1 `u`A fv_ve e2) {}N false) with ((cset_set (fv_ve e1) {}N false) `u` (cset_set (fv_ve e2) {}N false)).
-    + apply subset_union...
-    + unfold cset_union; simpl; rewrite empty_funion_idempotent; reflexivity.
+  - fsetdec.
+  - apply atomset_subset_union...
 Qed.
 
-Lemma free_for_cv_bound_typing : forall E e (x : atom) S,
-  typing E e S ->
-  x A`in` (free_for_cv e) ->
-  exists T, binds x (bind_typ T) E.
-Proof with eauto using wf_cset_over_union, cv_free_never_universal.
-  intros * Typ xIn.
-  induction Typ; simpl in *...
-  - assert (x = x0) by fsetdec; subst...
-  - assert (x = x0) by fsetdec; subst...
-  - pick fresh y.
-    forwards HA: H2 y.
-    + notin_solve.
-    + forwards (? & ? & ?): free_for_cv_open e1 0 y.
-      unfold open_ve.
-      clear Fr;fsetdec.
-    + destruct HA as (T & HA)...
-      inversion HA.
-      assert (x <> y) by notin_solve.
-      destruct (x == y)...
-      easy.
-  - destruct_union_mem xIn...
-  - pick fresh y.
-    destruct (cset_references_fvar_over_union _ _ _ xIn).
-    + apply IHTyp...
-    + forwards HA: H0 y.
-      * notin_solve.
-      * assert (cset_subset_prop (free_for_cv e) (free_for_cv (open_ve e y (`cset_fvar` y)))) by apply (free_for_cv_open e 0 y).
-        assert (cset_subset_prop (free_for_cv k) (free_for_cv (open_ve k y (`cset_fvar` y)))) by apply (free_for_cv_open k 0 y).
-        clear - xIn H1 H2 H3 IHTyp.
-        rewrite <- fvars_union_1 in xIn.
-        apply subset_in with (A := free_for_cv k)...
-      * destruct HA as (T & HA)...
-        inversion HA.
-        assert (x <> y) by notin_solve.
-        destruct (x == y)...
-        easy.
-  - pick fresh y.
-    forwards HA: H2 y.
-    + notin_solve.
-    + forwards (? & ? & ?): free_for_cv_open_type e1 0 y.
-      clear Fr;fsetdec.
-    + destruct HA as (T & HA)...
-      inversion HA.
-      assert (x <> y) by notin_solve.
-      destruct (x == y)...
-      easy.
+Lemma exp_cv_closed : forall e,
+  `cset_bvars` (exp_cv e) = {}N.
+Proof with eauto using var_cv_closed.
+  induction e; simpl...
+  - rewrite (var_cv_closed v), (var_cv_closed v0); csetdec.
+  - rewrite IHe1, IHe2; csetdec.
+  - rewrite (var_cv_closed v); csetdec.
 Qed.
+
+Lemma self_bound_impossible : forall X Γ,
+  Γ ⊢ wf ->
+  ~ bound X X Γ.
+Proof with eauto*.
+  intros.
+  induction H; intro.
+  - inversion H; inversion H0.
+  - inversion H2; inversion H3; destruct (X == X0); inversion H5; subst...
+    inversion H0; subst.
+    assert (X0 ∈ dom Γ) by (apply binds_In in H7; eauto* ).
+    apply (H1 H4).
+  - inversion H2; inversion H3; destruct (X == x); inversion H5; subst...
+    inversion H0; subst.
+    assert (x ∈ dom Γ) by (apply binds_In in H7; eauto* ).
+    apply (H1 H4).
+Qed.
+
+(* REVIEW: hard to prove *)
+Lemma wf_env_bound_to_var_implies_var_bind_sub : forall Γ x (X : atom),
+  Γ ⊢ wf ->
+  bound x X Γ ->
+  exists S, binds X (bind_sub S) Γ.
+Proof with eauto*.
+  intros.
+  generalize dependent X.
+  generalize dependent x.
+  induction H; intros.
+  - inversion H0; inversion H.
+  - inversion H2; subst.
+    + inversion H3; subst.
+      destruct (x == X); subst.
+      * inversion H5; subst.
+      * destruct (IHwf_env x X0 (bound_typ x X0 Γ H5)) as [S ?].
+        exists S.
+        assert (X0 <> X).
+        { pose proof (binds_In _ _ _ _ H4).
+          fsetdec.
+        }
+        apply binds_tail; simpl...
+    + inversion H3; subst.
+      destruct (x == X); subst.
+      * inversion H3; inversion H5; subst.
+        destruct (X == X0); subst.
+        -- admit.
+        -- admit.
+      * admit.
+Admitted.
+
+Lemma subcapt_empty : forall Γ C,
+  Γ ⊢ₛ C wf ->
+  Γ ⊢ₛ {} <: C.
+Proof with eauto*.
+  intros.
+  apply subcapt_set...
+  intros x xIn.
+  exfalso.
+  fsetdec.
+Qed.
+
+Lemma bound_in_wf_env_implies_wf_typ : forall Γ x T,
+  Γ ⊢ wf ->
+  bound x T Γ ->
+  Γ ⊢ T wf.
+Proof with eauto*.
+  intros.
+  induction H.
+  - inversion H0; inversion H.
+  - inversion H0; inversion H3; destruct (x == X); subst;
+    rewrite_env (∅ ++ [(X, bind_sub T0)] ++ Γ);
+    apply wf_typ_weakening; simpl_env...
+  - inversion H0; inversion H3; destruct (x == x0); subst;
+    rewrite_env (∅ ++ [(x0, bind_typ T0)] ++ Γ);
+    apply wf_typ_weakening; simpl_env...
+Qed.
+
+(*
+Lemma typing_var_bind_typ : forall Γ (x : atom) T,
+  Γ ⊢ x : T ->
+  exists S, Γ ⊢ S <: T /\ binds x (bind_typ S) Γ.
+Proof with eauto*.
+  intros.
+  dependent induction H.
+  - Case "typing_var_tvar".
+    exists (C # X).
+    split...
+    apply sub_capt...
+    + apply subcapt_empty.
+      apply wf_concrete_cset.
+      * intros y xIn; assert (y = x) by fsetdec; subst; clear xIn.
+        exists ({} # X).
+        apply bound_typ, H0.
+      * enough (x ∈ dom Γ) by fsetdec.
+        apply binds_In in H0; assumption.
+    + apply sub_refl_tvar...
+      assert (Γ ⊢ ({} # X) wf) by (apply bound_in_wf_env_implies_wf_typ with (x := x); eauto* ).
+      inversion H1; subst.
+      apply H6.
+  - Case "typing_var".  
+      * unfold wf_cset.
+        intros y x0In.
+        destruct (y == x); try (contradict n; fsetdec); subst.
+        exists X.
+        apply bound_typ, H0.
+      * enough (x ∈ dom Γ) by fsetdec.
+        eapply binds_In, H0.
+    + destruct (wf_env_bound_to_var_implies_var_bind_sub Γ x X H (bound_typ x X Γ H0)) as [S ?].
+      apply wf_typ_var with (T := S), H1.
+  - Case "typing_var".
+    exists (C # R).
+    split...
+    apply sub_capt.
+    + admit. (* REVIEW: unprovable *)
+    + admit. (* REVIEW: need reflexivity here which has not yet been proven *)
+  - Case "typing_sub".
+    admit.
+Admitted.*)
+
+(*
+Γ ⊢ e : T ->
+x ∈ fv_ve e ->
+exists S, binds x (bind_typ S) Γ.
+*)
 
 (** This should be easily true: free variables
     are all bound if a term has a type.... *)
-Lemma typing_cv : forall E e T,
-  typing E e T ->
-  wf_cset_in E (free_for_cv e).
-Proof with eauto using cv_free_never_universal, wf_cset_over_union; eauto*.
+Lemma typing_cv : forall Γ e T,
+  Γ ⊢ e : T ->
+  Γ ⊢ₛ (exp_cv e) wf.
+Proof with eauto using wf_cset_over_union; eauto*.
   intros * Htyp.
   induction Htyp; simpl...
-  (** TODO: merge the abs/t-abs case somehow (maybe a match to decide what
-      gets posed? )*)
-  - forwards: binds_In H0.
+  - Case "typing_var".
+    forwards: binds_In H0.
     simpl. constructor...
     intros y ?.
     assert (x = y) by fsetdec.
-    subst. exists X...
+    subst.
+    exists (C # R)...
     fsetdec.
-  - forwards: binds_In H0.
-    simpl. constructor...
-    intros y ?.
-    assert (x = y) by fsetdec.
-    subst. exists (typ_capt C P)...
-    fsetdec.
-  - pick fresh y.
+  - Case "typing_abs".
+    pick fresh y.
     assert (y `notin` L) by fsetdec.
-    assert (~ y A`in` (free_for_cv e1)). {
-      pose proof (free_for_cv_is_free_ve e1) as P...
-      inversion P; subst.
-      simpl in *.
-      csetdec.
-    }
-    forwards SpH0: H2 y...
-    pose proof (free_for_cv_open e1 0 y (`cset_fvar` y))...
-    pose proof (cv_free_never_universal).
-    pose proof (cv_free_is_bvar_free e1).
-    destruct (free_for_cv e1) eqn:Hfcv1; subst...
-    unfold open_ve in *.
-    inversion SpH0; subst...
-    assert (t0 = {}N) by fnsetdec; subst...
-    rename select (_ = _) into EQ.
-    rename select (cset_subset_prop _ _) into HH.
-    destruct HH as (HA1 & HA2 & HA3).
-    rewrite <- EQ in *.
-    simpl in *.
-    constructor.
-    2: clear Fr; fsetdec.
-    intros x ?.
-    destruct (x == y). {
-      csetdec.
-    }
-    forwards (T & B): H9 x. {
+    assert (~ y A`in` (exp_cv e1)).
+    { pose proof (exp_cv_subset_fv_ve e1) as P... }
+    forwards SpH0: H1 y...
+    pose proof (exp_cv_open_ve_rec e1 0 y (`cset_fvar` y))...
+    pose proof (exp_cv_closed e1).
+    destruct (exp_cv e1) eqn:Ecv1; subst.
+    inversion SpH0; subst.
+    unfold open_ve in H5.
+    rewrite <- H5 in H4.
+    destruct H4 as [t_sub_fvars [_ b_le_univ]].
+    econstructor.
+    + intros x xIn.
+      assert (x ∈ fvars) by (clear - xIn t_sub_fvars; fsetdec).
+      destruct (H6 x H4).
+      assert (x <> y) by (clear - xIn H3; fsetdec).
+      inversion H7; inversion H10; destruct (x == y)...
+    + clear - t_sub_fvars H3 H8.
+      simpl in H8.
       fsetdec.
-    }
-    simpl_env in *.
-    exists T. destruct_bound B; binds_cases B...
-  - apply wf_cset_over_union...
-  - (* typing_let *)
+  - Case "typing_app".
+    apply wf_cset_union...
+  - Case "typing_let".
     apply wf_cset_over_union; split...
     pick fresh y.
     assert (y `notin` L) by fsetdec.
-    assert (~ y A`in` (free_for_cv k)). {
-      pose proof (free_for_cv_is_free_ve k) as P...
-      inversion P; subst.
-      simpl in *.
-      csetdec.
-    }
+    assert (~ y A`in` (exp_cv k)).
+    { pose proof (exp_cv_subset_fv_ve k) as P... }
     forwards SpH0: H0 y...
-    pose proof (free_for_cv_open k 0 y (`cset_fvar` y))...
-    pose proof (cv_free_never_universal).
-    pose proof (cv_free_is_bvar_free k).
-    destruct (free_for_cv k) eqn:Hfcv1; subst...
+    pose proof (exp_cv_open_ve_rec k 0 y (`cset_fvar` y))...
+    pose proof (exp_cv_closed k).
+    destruct (exp_cv k) eqn:Hfcv1; subst...
     unfold open_ve in *.
     inversion SpH0; subst...
-    assert (t0 = {}N) by fnsetdec; subst...
     rename select (_ = _) into EQ.
     rename select (cset_subset_prop _ _) into HH.
     destruct HH as (HA1 & HA2 & HA3).
@@ -618,25 +767,20 @@ Proof with eauto using cv_free_never_universal, wf_cset_over_union; eauto*.
     destruct (x == y). {
       csetdec.
     }
-    forwards (T & B): H7 x. {
+    forwards (T & B): H5 x. {
       fsetdec.
     }
     simpl_env in *.
     exists T. destruct B as [B|B]; binds_cases B...
-  - (* typing_tapp *)
+  - Case "typing_tapp".
     pick fresh y.
     assert (y `notin` L) by fsetdec.
-    assert (~ y A`in` (free_for_cv e1)). {
-      pose proof (free_for_cv_is_free_ve e1) as P...
-      inversion P; subst.
-      simpl in *.
-      csetdec.
-    }
-    forwards SpH0: H2 y...
-    pose proof (free_for_cv_open_type e1 0 y)...
-    pose proof (cv_free_never_universal).
-    pose proof (cv_free_is_bvar_free e1).
-    destruct (free_for_cv e1) eqn:Hfcv1; subst...
+    assert (~ y A`in` (exp_cv e1)).
+    { pose proof (exp_cv_subset_fv_ve e1) as P... }
+    forwards SpH0: H1 y...
+    pose proof (exp_cv_open_te_rec e1 0 y)...
+    pose proof (exp_cv_closed e1).
+    destruct (exp_cv e1) eqn:Hfcv1; subst...
     unfold open_te in *.
     inversion SpH0; subst...
     rename select (_ = _) into EQ.
@@ -644,23 +788,26 @@ Proof with eauto using cv_free_never_universal, wf_cset_over_union; eauto*.
     rename select (cset_subset_prop _ _) into HH.
     destruct HH as (HA1 & HA2 & HA3).
     simpl in *.
-    assert (t0 = {}N) by fnsetdec; subst...
     constructor.
     2: clear Fr; fsetdec.
     intros x ?.
     destruct (x == y). {
       csetdec.
     }
-    forwards (T & B): H9 x. {
+    forwards (T & B): H6 x. {
       fsetdec.
     }
     simpl_env in *.
     exists T. destruct_bound B; binds_cases B...
-Qed.
+  - Case "typing_box".
+    apply wf_cset_union...
+    inversion H; subst.
+    apply wf_concrete_cset...
+Qed. 
 
 Lemma subst_cset_fresh_for_cv_var : forall z v C,
   z `notin` fv_vv v ->
-  subst_cset z C (free_for_cv_var v) = free_for_cv_var v.
+  subst_cset z C (var_cv v) = var_cv v.
 Proof with eauto*.
   intros.
   destruct v; unfold subst_cset; simpl in *...
@@ -672,7 +819,7 @@ Qed.
 
 Lemma subst_cset_fresh_for_cv : forall z t C,
   z `notin` fv_ve t ->
-  subst_cset z C (free_for_cv t) = free_for_cv t.
+  subst_cset z C (exp_cv t) = exp_cv t.
 Proof with eauto using subst_cset_fresh_for_cv_var; eauto*.
   intros.
   induction t; simpl in H |- *...
@@ -682,6 +829,17 @@ Proof with eauto using subst_cset_fresh_for_cv_var; eauto*.
     rewrite IHt1 by notin_solve.
     rewrite IHt2 by notin_solve.
     reflexivity.
+  - unfold subst_cset.
+    destruct_set_mem z {}A...
+    exfalso; clear - zIn; fsetdec.
+  - destruct c.
+    unfold subst_cset; simpl.
+    destruct_set_mem z (t `u`A `cset_fvars` (var_cv v))...
+    destruct (AtomSetNotin.elim_notin_union H).
+    destruct (AtomSet.F.union_1 zIn).
+    + exfalso; apply (H0 H2).
+    + rewrite cset_fvars_var_cv_is_fv_vv in H2.
+      exfalso; apply (H1 H2).
 Qed.
 
 (*
@@ -744,144 +902,65 @@ Proof with eauto.
 Qed.
 *)
 
-Lemma subst_te_idempotent_wrt_free_for_cv : forall e x C,
-  free_for_cv (subst_te x C e) = free_for_cv e.
-Proof with eauto.
-  intros.
-  induction e; simpl...
-  rewrite IHe1, IHe2...
-Qed.
-
-Lemma bind_typ_notin_fv_tt : forall x S E Ap Am T,
-  binds x (bind_typ S) E ->
-  wf_typ E Ap Am T ->
-  x `~in`A fv_tt T
-with bind_typ_notin_fv_tpt : forall x S E Ap Am T,
-  binds x (bind_typ S) E ->
-  wf_pretyp E Ap Am T ->
-  x `~in`A fv_tpt T.
+Lemma bind_typ_notin_fv_tt : forall x S Γ T,
+  binds x (bind_typ S) Γ ->
+  Γ ⊢ T wf ->
+  x `~in`A fv_tt T.
 Proof with auto.
-{ intros * Hbnd WfT.
-  dependent induction T;simpl...
-  - inversion WfT; subst.
-    eapply bind_typ_notin_fv_tpt; eauto.
-  - inversion WfT; subst.
-    destruct (x == a); [|fsetdec].
-    subst.
-    forwards: binds_unique a; eauto.
-}
-{ intros * Hbnd WfT.
-  dependent induction T; simpl.
-  - fsetdec.
-  - inversion WfT; subst.
-    rename H4 into Wf__t.
-    rename H5 into Wf__t0.
-    pick fresh y.
-    specialize (Wf__t0 y ltac:(fsetdec)).
-    forwards: bind_typ_notin_fv_tt Wf__t; [eauto|..].
-    forwards HA: bind_typ_notin_fv_tt x Wf__t0; [eauto|..].
-    forwards: notin_fv_tt_open_ct HA.
-    notin_solve.
-  - inversion WfT; subst.
-    rename H4 into Wf__t.
-    rename H5 into Wf__t0.
-    pick fresh y.
-    specialize (Wf__t0 y ltac:(fsetdec)).
-    forwards: bind_typ_notin_fv_tt Wf__t; [eauto|..].
-    forwards HA: bind_typ_notin_fv_tt x Wf__t0; [eauto|..].
-    forwards: notin_fv_tt_open_tt HA.
-    notin_solve.
-}
+  intros * Hbnd WfT.
+  dependent induction WfT; simpl...
+  - apply AtomSetNotin.notin_union...
+    pick fresh y and specialize H0.
+    eapply notin_fv_tt_open_ct with (C := `cset_fvar` y).
+    apply H0.
+    apply binds_tail...
+  - apply AtomSetNotin.notin_union...
+    pick fresh Y and specialize H1.
+    eapply notin_fv_tt_open_tt.
+    apply H1.
+    apply binds_tail...
 Qed.
 
-Lemma wf_cset_notin_fvars : forall x E A C,
-  wf_cset E A C ->
-  x `~in`A dom E ->
+Lemma wf_cset_notin_fvars : forall x Γ C,
+  Γ ⊢ₛ C wf ->
+  x `~in`A dom Γ ->
   x `~in`A (`cset_fvars` C).
 Proof with eauto*.
   intros * WfC NotIn.
   induction WfC.
-  enough (fvars `c`A dom E) by fsetdec.
+  enough (fvars `c`A dom Γ) by fsetdec.
   intros y yIn.
   destruct (H y ltac:(fsetdec)) as [T [B|B]]; eapply binds_In...
 Qed.
 
-Lemma wf_typ_notin_fv_ct : forall x E Ap Am T,
-  wf_typ E Ap Am T ->
-  x `~in`A dom E ->
-  x `~in`A fv_ct T
-with wf_pretyp_notin_fv_cpt : forall x E Ap Am P,
-  wf_pretyp E Ap Am P ->
-  x `~in`A dom E ->
-  x `~in`A fv_cpt P.
+Lemma wf_typ_notin_fv_ct : forall x Γ T,
+  Γ ⊢ T wf ->
+  x `~in`A dom Γ ->
+  x `~in`A fv_ct T.
 Proof with eauto*.
-{ intros * WfT NotIn.
+  intros * WfT NotIn.
   induction WfT; simpl.
   - fsetdec.
-  - assert (x `~in`A (`cset_fvars` C)) by (applys wf_cset_notin_fvars; eauto*).
-    assert (x `~in`A fv_cpt P) by (applys wf_pretyp_notin_fv_cpt; eauto*).
-    fsetdec.
-}
-{ intros * WfP NotIn.
-  induction WfP; simpl.
   - fsetdec.
-  - assert (x `~in`A fv_ct T1) by (applys wf_typ_notin_fv_ct; eauto*).
+  - apply AtomSetNotin.notin_union...
     pick fresh y and specialize H0.
-    assert (x `~in`A fv_ct T2).
-    { eapply notin_fv_ct_open_ct.
-      eapply wf_typ_notin_fv_ct.
-      apply H0.
-      simpl.
-      assert (x <> y) by (clear - Fr; fsetdec).
-      clear Fr.
-      fsetdec.
-    }
-    clear - H1 H2.
-    fsetdec.
-  - assert (x `~in`A fv_ct T1) by (applys wf_typ_notin_fv_ct; eauto*).
-    pick fresh y and specialize H0.
-    assert (x `~in`A fv_ct T2).
-    { eapply notin_fv_ct_open_tt.
-      eapply wf_typ_notin_fv_ct.
-      apply H0.
-      simpl.
-      assert (x <> y) by (clear - Fr; fsetdec).
-      clear Fr.
-      fsetdec.
-    }
-    clear - H1 H2.
-    fsetdec.
-}
-Qed.
-
-Lemma wf_typ_in_notin_fv_ct : forall x E T,
-  wf_typ_in E T ->
-  x `~in`A dom E ->
-  x `~in`A fv_ct T
-with wf_pretyp_in_notin_fv_cpt : forall x E P,
-  wf_pretyp_in E P ->
-  x `~in`A dom E ->
-  x `~in`A fv_cpt P.
-Proof with eauto*.
-{ intros * WfT NotIn.
-  eapply wf_typ_notin_fv_ct with (E := E) (Ap := dom E) (Am := dom E)...
-}
-{ intros * WfP NotIn.
-  eapply wf_pretyp_notin_fv_cpt with (E := E) (Ap := dom E) (Am := dom E)...
-}
+    apply notin_fv_ct_open_ct with (C := `cset_fvar` y)...
+  - apply AtomSetNotin.notin_union...
+    pick fresh Y and specialize H1.
+    apply notin_fv_ct_open_tt with (U := Y)...
+  - apply (IHWfT NotIn).
+  - apply AtomSetNotin.notin_union...
+    eapply wf_cset_notin_fvars...
 Qed.
 
 (* ********************************************************************** *)
 (** * #<a name="regularity"></a># Regularity of relations *)
 
-Lemma subcapt_regular : forall E C D,
-  subcapt E C D ->
-  wf_cset_in E C /\ wf_cset_in E D.
+Lemma subcapt_regular : forall Γ C D,
+  Γ ⊢ₛ C <: D ->
+  Γ ⊢ₛ C wf /\ Γ ⊢ₛ D wf.
 Proof with eauto*.
-  (* Useful when copying this lemma to definitions. *)
-  Require Import Program.Equality.
-  Require Import TaktikZ.
-  intros* H.
+  intros * H.
   dependent induction H; subst...
   - split...
     constructor.
@@ -913,44 +992,42 @@ Proof with eauto*.
       fsetdec.
 Qed.
 
-(* TODO check whether we need those and otherwise drop *)
-Hint Unfold wf_typ_in : core.
-Hint Unfold wf_pretyp_in : core.
-
-Lemma sub_regular : forall E S T,
-  sub E S T ->
-  wf_env E /\ wf_typ_in E S /\ wf_typ_in E T
-with sub_pre_regular : forall E S T,
-  sub_pre E S T ->
-  wf_env E /\ wf_pretyp_in E S /\ wf_pretyp_in E T.
+Lemma sub_regular : forall Γ S T,
+  Γ ⊢ S <: T ->
+  Γ ⊢ wf /\ Γ ⊢ S wf /\ Γ ⊢ T wf.
 Proof with simpl_env; eauto*.
-------
-  intros E S T H.
-  induction H.
-  - repeat split...
-  - Case "sub_trans_tvar".
-    repeat split...
-    apply wf_typ_var with (U := U)...
-    eapply binds_In...
+  intros.
+  induction H...
   - Case "sub_capt".
-    assert (wf_cset_in E C1 /\ wf_cset_in E C2). { apply subcapt_regular... }
-    assert (wf_env E /\ wf_pretyp_in E P1 /\ wf_pretyp_in E P2). { apply sub_pre_regular... }
+    destruct (subcapt_regular _ _ _ H).
     repeat split...
-------
-  intros E S T H.
-  induction H.
-  - repeat split...
-  - Case  "sub_trans_arrow".
-    pose proof (sub_regular E _ _ H).
-    repeat split; [
-      auto* |
-      apply wf_typ_arrow with (L := L); auto* |
-      apply wf_typ_arrow with (L := L); auto*
-    ].
+    + constructor...
+      admit.
+    + constructor...
+      admit.
+  - Case "sub_arr".
+    repeat split...
+    + pick fresh x and apply wf_typ_arr...
+      apply H1.
+      fsetdec.
+    + pick fresh x and apply wf_typ_arr...
+      rewrite_env (∅ ++ [(x, bind_typ S2)] ++ Γ).
+      eapply wf_typ_ignores_typ_bindings.
+      apply H1.
+      fsetdec.
   - Case "sub_all".
-    pose proof (sub_regular E _ _ H).
     repeat split...
-Qed.
+    + pick fresh X and apply wf_typ_all...
+      * admit.
+      * apply H1.
+        fsetdec.
+    + pick fresh X and apply wf_typ_all...
+      * admit.
+      * rewrite_env (∅ ++ [(X, bind_sub R2)] ++ Γ).
+        eapply wf_typ_ignores_sub_bindings.
+        apply H1.
+        fsetdec.
+Admitted.
 
 Lemma typing_var_implies_binds : forall E (x : atom) T,
   typing E x T ->
@@ -960,31 +1037,26 @@ Proof with eauto*.
   dependent induction Typ...
 Qed.
 
-Lemma typing_regular : forall E e T,
-  typing E e T ->
-  wf_env E /\ expr e /\ wf_typ_in E T.
+Lemma typing_regular : forall Γ e T,
+  Γ ⊢ e : T ->
+  Γ ⊢ wf /\ expr e /\ Γ ⊢ T wf.
 Proof with simpl_env; auto*.
   intros * H.
-  induction H...
-  (* typing rule: x : X \in E --> E |- x : X *)
-  - repeat split...
-    apply wf_typ_from_binds_typ with (x := x)...
-  (* typing rule : x : C P \in E --> E |- x : {x} P *)
-  - repeat split...
-    assert (wf_typ_in E (typ_capt C P)). {
-      apply wf_typ_from_binds_typ with (x := x)...
-    }
-    inversion H1; subst...
+  induction H.
+  - Case "typing_var".
+    repeat split...
+    assert (WfCR : Γ ⊢ (C # R) wf) by (apply bound_in_wf_env_implies_wf_typ with (x := x); auto).
+    inversion WfCR; subst...
     constructor...
-    constructor...
-    + intros y ?.
-      assert (y = x) by fsetdec; subst; eauto.
-    + assert (x `in` dom E).
-      2: fsetdec.
-      eapply binds_In; eauto.
-  (* typing rule: (\x e) has type fv((\x e)) T1 -> T2 *)
-  - pick fresh y; assert (y `notin` L) by fsetdec...
-    unshelve epose proof (H2 y _) as H4...
+    constructor.
+    + intros y yIn; destruct (y == x); try (contradict n; fsetdec); subst; clear yIn.
+      exists (C # R).
+      apply bound_typ, H0.
+    + enough (x ∈ dom Γ) by fsetdec.
+      apply binds_In in H0...
+  - Case "typing_abs".
+    pick fresh y; assert (y `notin` L) by fsetdec...
+    unshelve epose proof (H1 y _) as H4...
     inversion H4 as [Henv [Hexpr Hwf]]...
     repeat split...
     + inversion Henv...
@@ -992,77 +1064,83 @@ Proof with simpl_env; auto*.
       * eapply type_from_wf_typ.
         eapply wf_typ_from_wf_env_typ.
         apply Henv.
-      * destruct (H2 x)...
+      * destruct (H1 x)...
     + constructor...
-      eapply typing_cv with (e := (exp_abs V e1)) (T := (typ_capt (free_for_cv e1) (typ_arrow V T1)))...
+      eapply typing_cv with (e := (exp_abs V e1)) (T := exp_cv e1 # ∀ (V) T1)...
       * apply typing_abs with (L := L)...
-      * eapply wf_typ_arrow; trivial.
-        apply H0.
-  (* typing rule: application *)
-  - repeat split...
+      * eapply wf_typ_arr; trivial.
+        apply H1.
+      * apply type_from_wf_typ in H.
+        pick fresh x and apply type_arr...
+        eapply type_from_wf_typ with (Γ := [(x, bind_typ V)] ++ Γ).
+        apply H1.
+        fsetdec.
+  - Case "typing_app".
     destruct IHtyping1 as [_ [_ Hwf]].
-    inversion Hwf; subst...
-    apply wf_typ_set_weakening with (Ap := dom E) (Am := dom E)...
-    (** needs substitution lemma here. *)
-    apply wf_typ_open_capt with (T1 := T1)...
+    inversion Hwf; inversion H5; subst...
+    repeat split...
+    apply wf_typ_open_capt with (S := T1)...
     destruct (typing_var_implies_binds _ _ _ H0) as [T1' xBinds].
     constructor.
     + intros z zIn; assert (z = x) by (clear - zIn; fsetdec); subst; clear zIn.
       eauto.
-    + enough (x `in`A dom E) by fsetdec.
+    + enough (x `in`A dom Γ) by fsetdec.
       eapply binds_In, xBinds.
-  (* typing rule: let *)
-  - repeat split...
+  - Case "typing_let".
+    repeat split...
     + pick fresh x and apply expr_let...
       assert (x `notin` L) by fsetdec...
       unshelve epose proof (H1 x _) as H3...
     + pick fresh x.
       destruct (H1 x ltac:(fsetdec)) as [_ [_ wf_T2]].
-      assert (wf_typ E (dom ([(x, bind_typ T1)] ++ E) `\`A x) (dom ([(x, bind_typ T1)] ++ E) `\`A x) T2).
-      { unfold wf_typ_in in wf_T2; simpl in *; simpl_env in *.
-        rewrite_env (empty ++ E).
-        eapply wf_typ_strengthen_typ with (x := x) (U := T1)...
-        replace ({}A `u`A dom E) with (dom E) by (clear; fsetdec).
-        apply wf_T2.
+      assert (Γ ⊢ T2 wf).
+      { rewrite_env (∅ ++ Γ).
+        eapply wf_typ_strengthen with (x := x) (U := T1)...
       }
-      assert (dom ([(x, bind_typ T1)] ++ E) `\`A x = dom E).
-      { clear - x T1 E Fr.
-        assert (x `~in`A dom E) by fsetdec.
-        clear Fr.
-        simpl. fsetdec.
-      }
-      rewrite H3 in H2.
       apply H2.
-  (* typing rule: type abstractions. *)
-  - pick fresh y; assert (y `notin` L) by fsetdec...
-    unshelve epose proof (H2 y _) as H4...
-    inversion H4 as [Henv [Hexpr _]]...
+  - Case "typing_tabs".
+    pick fresh Y; assert (Y `notin` L) by fsetdec...
+    unshelve epose proof (H1 Y _) as H4...
+    inversion H4 as [Henv [Hexpr Hwf]]...
     repeat split...
     + inversion Henv...
-    + pick fresh x and apply expr_tabs.
-      * eapply type_from_wf_typ.
-        eapply wf_typ_from_wf_env_sub.
-        apply Henv.
-      * destruct (H2 x)...
+    + pick fresh X and apply expr_tabs.
+      * admit.
+      * destruct (H1 X)...
     + constructor...
-      apply typing_cv with (e := (exp_tabs V e1)) (T := (typ_capt (free_for_cv e1) (typ_all V T1)))...
-      apply typing_tabs with (L := L)...
-      eapply wf_typ_all. assumption.
-      intros X XNotIn.
-      replace (dom E `u`A {X}A) with (dom ([(X, bind_sub V)] ++ E)).
-      * apply H2, XNotIn.
-      * simpl; clear; fsetdec.
-  (* typing rule: type application *)
-  - destruct IHtyping as [HwfE [Hexpr Hwf]]...
+      eapply typing_cv with (e := (exp_tabs V e1)) (T := exp_cv e1 # ∀ [V] T1)...
+      * apply typing_tabs with (L := L)...
+      * eapply wf_typ_all; trivial.
+        -- admit.
+        -- apply H1.
+      * apply type_from_wf_typ in H.
+        pick fresh X and apply type_all...
+        -- admit.
+        -- eapply type_from_wf_typ with (Γ := [(X, bind_sub V)] ++ Γ).
+           apply H1.
+           fsetdec.
+  - Case "typing_tapp".
+    destruct IHtyping as [HwfΓ [Hexpr Hwf]]...
     forwards (R1 & R2 & R3): sub_regular H0...
     repeat split...
     + constructor...
-      eapply type_from_wf_typ with (E := E); apply R2.
-    + apply wf_typ_open_type with (T1 := T1)...
-      inversion Hwf; subst...
-  - repeat split...
-    forwards: sub_regular H0...
-Qed.
+      eapply type_from_wf_typ with (Γ := Γ); apply R2.
+    + apply wf_typ_open_type with (R := T1)...
+      * inversion Hwf; subst...
+      * admit.
+  - Case "typing_box".
+    repeat split...
+  - Case "typing_unbox".
+    destruct IHtyping as [HwfΓ [Hex Hwf]].
+    inversion Hwf; inversion H3; subst.
+    repeat split...
+    apply expr_unbox.
+    eapply capt_from_wf_cset, H0.
+  - Case "typing_sub".
+    destruct IHtyping as [HwfΓ [Hex Hwf]].
+    repeat split...
+    applys sub_regular H0.
+Admitted.
 
 Lemma value_regular : forall e,
   value e ->
@@ -1071,9 +1149,9 @@ Proof.
   intros e H. induction H; auto.
 Qed.
 
-Lemma eval_typing_regular : forall E K T U,
-  eval_typing E K T U ->
-  wf_env E /\ wf_typ_in E T /\ wf_typ_in E U.
+Lemma eval_typing_regular : forall Γ K T U,
+  Γ ⊢ K : T ⇒ U ->
+  Γ ⊢ wf /\ Γ ⊢ T wf /\ Γ ⊢ U wf.
 Proof with eauto*.
   intros * EvalTyp.
   induction EvalTyp.
@@ -1083,6 +1161,57 @@ Proof with eauto*.
     destruct (typing_regular _ _ _ H) as [wf_xTE _].
     inversion wf_xTE; subst...
 Qed.
+
+Lemma exp_cv_bound_typing : forall Γ e (x : atom) S,
+  Γ ⊢ e : S ->
+  x A`in` (exp_cv e) ->
+  exists T, binds x (bind_typ T) Γ.
+Proof with eauto using wf_cset_over_union.
+  intros * Typ xIn.
+  induction Typ; simpl in *...
+  - assert (x = x0) by fsetdec; subst...
+  - pick fresh y.
+    forwards HA: H1 y.
+    + notin_solve.
+    + forwards (? & ? & ?): exp_cv_open_ve_rec e1 0 y.
+      unfold open_ve.
+      clear Fr;fsetdec.
+    + destruct HA as (T & HA)...
+      inversion HA.
+      assert (x <> y) by notin_solve.
+      destruct (x == y)...
+      easy.
+  - destruct_union_mem xIn...
+  - pick fresh y.
+    destruct (cset_references_fvar_over_union _ _ _ xIn).
+    + apply IHTyp...
+    + forwards HA: H0 y.
+      * notin_solve.
+      * assert (cset_subset_prop (exp_cv e) (exp_cv (open_ve e y (`cset_fvar` y)))) by apply (exp_cv_open_ve_rec e 0 y).
+        assert (cset_subset_prop (exp_cv k) (exp_cv (open_ve k y (`cset_fvar` y)))) by apply (exp_cv_open_ve_rec k 0 y).
+        clear - xIn H1 H2 H3 IHTyp.
+        rewrite <- fvars_union_1 in xIn.
+        apply subset_in with (A := exp_cv k)...
+      * destruct HA as (T & HA)...
+        inversion HA.
+        assert (x <> y) by notin_solve.
+        destruct (x == y)...
+        easy.
+  - pick fresh y.
+    forwards HA: H1 y.
+    + notin_solve.
+    + forwards (? & ? & ?): exp_cv_open_te_rec e1 0 y.
+      clear Fr;fsetdec.
+    + destruct HA as (T & HA)...
+      inversion HA.
+      assert (x <> y) by notin_solve.
+      destruct (x == y)...
+      easy.
+  - exfalso; clear - xIn; fsetdec.
+  - inversion Typ; subst.
+    destruct (AtomSet.F.union_1 xIn)...
+    admit. 
+Admitted.
 
 (* *********************************************************************** *)
 (** * #<a name="auto"></a># Automation *)
@@ -1110,7 +1239,7 @@ Qed.
     The other three hints try outright to solve their respective
     goals. *)
 
-Hint Extern 1 (wf_cset ?E _ ?C) =>
+Hint Extern 1 (wf_cset ?E ?C) =>
   match goal with
   | H: subcapt _ C _ |- _ => apply (proj1 (subcapt_regular _ _ _ H))
   | H: subcapt _ _ C |- _ => apply (proj2 (subcapt_regular _ _ _ H))
@@ -1120,23 +1249,15 @@ Hint Extern 1 (wf_cset ?E _ ?C) =>
 Hint Extern 1 (wf_env ?E) =>
   match goal with
   | H: sub _ _ _ |- _ => apply (proj1 (sub_regular _ _ _ H))
-  | H: sub_pre _ _ _ |- _ => apply (proj1 (sub_pre_regular _ _ _ H))
   | H: typing _ _ _ _ |- _ => apply (proj1 (typing_regular _ _ _ _ H))
   end
 : core.
 
-Hint Extern 1 (wf_typ ?E _ _ ?T) =>
+Hint Extern 1 (wf_typ ?E ?T) =>
   match goal with
   | H: typing E _ _ T |- _ => apply (proj2 (proj2 (typing_regular _ _ _ _ H)))
   | H: sub E T _ |- _ => apply (proj1 (proj2 (sub_regular _ _ _ H)))
   | H: sub E _ T |- _ => apply (proj2 (proj2 (sub_regular _ _ _ H)))
-  end
-: core.
-
-Hint Extern 1 (wf_pretyp ?E ?T) =>
-  match goal with
-  | H: sub_pre E T _ |- _ => apply (proj1 (proj2 (sub_pre_regular _ _ _ H)))
-  | H: sub_pre E _ T |- _ => apply (proj2 (proj2 (sub_pre_regular _ _ _ H)))
   end
 : core.
 
@@ -1150,21 +1271,12 @@ Hint Extern 1 (type ?T) =>
   end
 : core.
 
-Hint Extern 1 (pretype ?T) =>
-  let go E := eapply (pretype_from_wf_pretyp E); eauto in
-  match goal with
-  | H: sub_pre ?E T _ |- _ => go E
-  | H: sub_pre ?E _ T |- _ => go E
-  | H: wf_pretyp ?E _ _ T |- _ => go E
-  end
-: core.
-
 Hint Extern 1 (capt ?C) =>
   let go E := eapply (capt_from_wf_cset E); eauto in
   match goal with
   | H: subcapt ?E C _ |- _ => go E
   | H: subcapt ?E _ C |- _ => go E
-  | H: cv ?E _ C |- _ => go E
+  | H: exp_cv ?E _ C |- _ => go E
   end
 : core.
 
@@ -1176,27 +1288,11 @@ Hint Extern 1 (expr ?e) =>
   end
 : core.
 
-Hint Extern 1 (wf_pretyp ?E (dom ?E) (dom ?E) ?P) =>
-match goal with
-| H : typing E _ (typ_capt _ P) |- _ =>
-  apply typing_regular in H;
-  destruct H as [_ [_ H]];
-  inversion H; subst; assumption
-end : core.
-
-Hint Extern 1 (wf_pretyp_in ?E ?P) =>
-match goal with
-| H : typing E _ (typ_capt _ P) |- _ =>
-  apply typing_regular in H;
-  destruct H as [_ [_ H]];
-  inversion H; subst; assumption
-end : core.
-
 (** * #<a name="auto"></a># Automation Tests *)
 
-Local Lemma test_subcapt_regular : forall E C1 C2,
-  subcapt E C1 C2 ->
-  wf_cset E (dom E) C1 /\ wf_cset E (dom E) C2.
+Local Lemma test_subcapt_regular : forall Γ C1 C2,
+  Γ ⊢ₛ C1 <: C2 ->
+  Γ ⊢ₛ C1 wf /\ Γ ⊢ₛ C2 wf.
 Proof with eauto*.
   intros.
   repeat split.
